refactored primitive instruction invocatinos, patched proofs, also changed deprecated omega to lia for Coq 8.12 update

MonadVM.v
@@ -102,6 +102,8 @@ Definition add_trace (tr':list Ev) : vm_st -> vm_st :=
 
 Definition add_tracem (tr:list Ev) : VM unit :=
   modify (add_trace tr).
+Check modify.
+Print modify.
 
 Definition split_evm (i:nat) (sp1 sp2:SP) (e:EvidenceC) (p:Plc) : VM (EvidenceC*EvidenceC) :=
     let e1 := splitEv sp1 e in
@@ -109,11 +111,226 @@ Definition split_evm (i:nat) (sp1 sp2:SP) (e:EvidenceC) (p:Plc) : VM (EvidenceC*
     add_tracem [Term.split i p] ;;
                ret (e1,e2).
 
+(*
+Definition prim_trace (i:nat) (p:Plc) (a:Prim_Instr) : (list Ev) :=
+  match a with
+  | copy => [Term.copy i p]
+  | umeas asp_id => [Term.umeas i p asp_id]
+  | sign => [Term.sign i p]
+  | hash => [Term.hash i p]
+  end.
+ *)
+
+(*
+Definition prim_ev (a:Prim_Instr)(* (p:Plc) *) (e:EvidenceC) : EvidenceC :=
+  match a with
+  | copy => e
+  | umeas i =>
+    let bs := invokeUSM i in
+    (uuc i bs e)
+  | sign =>
+    let bs := signEv e in
+    (ggc bs e)
+  | hash =>
+    let bs := hashEv e in
+    (hhc bs e)
+  end. 
+*)
+
+(** * Place-holder axioms for IO operations *)
+(* Definition invokeKIM (i:ASP_ID) (q:Plc) (*(args:list Arg)*) : BS. 
+Admitted. *)
+Print BS.
+Definition BS_res : BS.
+Admitted.
+
+Check put_ev.
+
+Definition invokeUSM (x:nat) (i:ASP_ID) (p:Plc) : VM EvidenceC :=
+  e <- get_ev ;;
+  add_tracem [Term.umeas x p i];;
+  ret (uuc i BS_res e).
+
+Definition signEv (x:nat) (p:Plc) : VM EvidenceC :=
+  e <- get_ev ;;
+  add_tracem [Term.sign x p] ;;
+  ret (ggc BS_res e).
+
+Definition hashEv (x:nat) (p:Plc) : VM EvidenceC :=
+  e <- get_ev ;;
+  add_tracem [Term.hash x p] ;;
+  ret (hhc BS_res e).
+
+Definition copyEv (x:nat) (p:Plc) : VM EvidenceC :=
+  add_tracem [Term.copy x p] ;;
+  get_ev.
+
+Definition toRemote (t:Term) (pTo:Plc) (e:EvidenceC) : EvidenceC.
+Admitted.
+Definition parallel_eval_thread (t:Term) (e:EvidenceC) : EvidenceC.
+Admitted.
+
+Definition do_prim (x:nat) (p:Plc) (a:Prim_Instr) : VM EvidenceC :=
+  match a with
+  | copy => copyEv x p
+  | umeas asp_id =>
+    invokeUSM x asp_id p
+  | sign => signEv x p
+  | hash => hashEv x p
+  end.
+
+
+
+Definition eval_asp (a:ASP) (e:EvidenceC) : EvidenceC :=
+  match a with
+  | CPY => e
+(*  | KIM i q args =>
+    let bs := invokeKIM i q args in
+    (kkc i args q bs e) *)
+  | ASPC i =>
+    let bs := BS_res in
+    (uuc i bs e)
+  | SIG =>
+    let bs := BS_res in
+    (ggc bs e)
+  | HSH =>
+    let bs := BS_res in
+    (hhc bs e)
+  end.
+
+
+
+Fixpoint eval (t:Term) (* (p:Plc) *) (e:EvidenceC) : EvidenceC :=
+  match t with
+  | asp a => eval_asp a e
+  | att q t1 => toRemote t1 q e
+  | lseq t1 t2 =>
+    let e1 := eval t1 e in
+    eval t2 e1
+         
+  | bseq (sp1,sp2) t1 t2 =>
+    let e1 := splitEv sp1 e in
+    let e2 := splitEv sp2 e in
+    let e1' := eval t1 e1 in
+    let e2' := eval t2 e2 in
+    (ssc e1' e2') 
+  | bpar (sp1,sp2) t1 t2 =>
+    let e1 := splitEv sp1 e in
+    let e2 := splitEv sp2 e in
+    let e1' := parallel_eval_thread t1 e1 in
+    let e2' := parallel_eval_thread t2 e2 in
+    (ppc e1' e2')
+  end.
+
+
+
+Axiom remote_eval : forall e p annt,
+    eval annt e = toRemote annt p e.
+
+Axiom para_eval_thread: forall e annt,
+    parallel_eval_thread annt e = eval annt e.
+
+
+Inductive evalR: Term -> EvidenceC -> EvidenceC -> Prop :=
+| mttc: forall e, evalR (asp CPY) e e
+| uutc: forall i e,
+    evalR (asp (ASPC i)) e (uuc i (BS_res) e)
+| ggtc: forall e,
+    evalR (asp SIG) e (ggc BS_res e)
+| hhtc: forall e,
+    evalR (asp HSH) e (hhc BS_res e)
+| atc: forall q t' e e',
+    evalR t' e e' ->
+    evalR (att q t') e e'
+| lseqc: forall t1 t2 e e' e'',
+    evalR t1 e e' ->
+    evalR t2 e' e'' ->
+    evalR (lseq t1 t2) e e''
+| bseqc: forall t1 t2 sp1 sp2 e e1 e2,
+    evalR t1 (splitEv sp1 e) e1 ->
+    evalR t2 (splitEv sp2 e) e2 ->
+    evalR (bseq (sp1,sp2) t1 t2) e (ssc e1 e2)
+| bparc: forall t1 t2 sp1 sp2 e e1 e2,
+    evalR t1 (splitEv sp1 e) e1 ->
+    evalR t2 (splitEv sp2 e) e2 ->
+    evalR (bpar (sp1,sp2) t1 t2) e (ppc e1 e2).
+
+
+
+Lemma eval_iff_evalR: forall t e e',
+    evalR t e e' <-> eval t e = e'.
+Proof.
+    split.
+  - (* -> case *)
+    intros.
+    generalize dependent e.
+    generalize dependent e'.
+
+    induction t; intros.
+
+    (*
+    + destruct a; try (inv H; reflexivity).
+    + inv H. simpl.
+      rewrite <- remote_eval.
+      eauto.
+    + inv H.
+      assert (eval t1 e = e'0).
+      eauto.
+      subst.
+      simpl.
+      eauto.
+    + inv H.
+      assert (eval t1 (splitEv sp1 e) = e1) by eauto.
+      assert (eval t2 (splitEv sp2 e) = e2) by eauto.
+      simpl.
+      destruct sp1; destruct sp2;
+        simpl; subst; eauto.
+    + inv H.
+      assert (eval t1 (splitEv sp1 e) = e1) by eauto.
+      assert (eval t2 (splitEv sp2 e) = e2) by eauto.
+      simpl.
+      repeat rewrite para_eval_thread in *.
+      destruct sp1; destruct sp2;
+        simpl; subst; eauto.
+  - (* <- case *)
+    intros.
+    generalize dependent e.
+    generalize dependent e'.
+
+    induction t; intros.
+    + inv H.
+      destruct a; try econstructor.
+    + inv H.
+      simpl.
+      econstructor.
+      rewrite <- remote_eval.
+      eauto.
+    + econstructor; eauto.
+    + destruct s.
+      simpl in H.
+      destruct s; destruct s0; simpl in *; subst;
+        econstructor; (try simpl); eauto; try (econstructor).
+    + destruct s.
+      simpl in H.
+      repeat rewrite para_eval_thread in *.
+      destruct s; destruct s0; simpl in *; subst;
+        econstructor; (try simpl); eauto; try (econstructor).
+Defined.
+     *)
+Admitted.
+
        
 Ltac monad_unfold :=
   repeat unfold
          runSt,
   execSt,
+  
+  do_prim,
+  invokeUSM,
+  signEv,
+  hashEv,
+  copyEv,
+  
   (*push_stackm,
   pop_stackm, *)
   (*push_stack,
